src/SoftBound/sb_pp.v
@@ -21,6 +21,7 @@ Require Import Memdata.
 Require Import Memory.
 Require Import Integers.
 Require Import sb_tactic.
+Require Import symexe_def.
 
 Import SoftBound.
 
@@ -29,7 +30,7 @@ Definition wf_data (TD:TargetData) (M:mem) (gvb gve:GenericValue) : Prop :=
          GV2ptr TD (getPointerSize TD) gve) with
   | (Some (Values.Vptr bb bofs), Some (Values.Vptr eb eofs)) =>
       if zeq bb eb then
-        Mem.range_perm M bb (Int.signed 31 bofs) (Int.signed 31 eofs) Readable
+        Mem.range_perm M bb (Int.signed 31 bofs) (Int.signed 31 eofs) Writable
       else False
   | _ => False
   end.
@@ -53,23 +54,23 @@ Lemma range_perm_alloc_other:
   Mem.range_perm m2 b' lo' hi' p.
 Proof.
   intros. inv H. red.
-Admitted.
+Admitted. (* mem *)
 
 Lemma store_range_perm_1:
   forall chunk m1 b ofs v m2, Mem.store chunk m1 b ofs v = Some m2 ->
   forall b' lo' hi' p,
   Mem.range_perm m1 b' lo' hi' p -> Mem.range_perm m2 b' lo' hi' p.
-Admitted.
+Admitted. (* mem *)
 
 Lemma GV2ptr_base2GV : forall TD mb,
   GV2ptr TD (getPointerSize TD) (base2GV TD mb) = 
     Some (Values.Vptr mb (Int.repr 31 0)).
-Admitted.
+Admitted. (* could be wrong *)
 
 Lemma GV2ptr_bound2GV : forall TD mb tsz n,
   GV2ptr TD (getPointerSize TD) (bound2GV TD mb tsz n) = 
     Some (Values.Vptr mb (Int.repr 31 ((Size.to_Z tsz)*n))).
-Admitted.
+Admitted. (* could be wrong *)
 
 Lemma wf_mmetadata__wf_data : forall Mem0 TD MM b0 ofs gvb gve,
   wf_mmetadata TD Mem0 MM ->
@@ -108,26 +109,117 @@ Proof.
   eapply wf_data__store__wf_data; eauto.
 Qed.
 
+Lemma wf_rmetadata__get_const_metadata_aux : forall TD Mem0 gl t i0 gvb gve,
+  const2GV TD Mem0 gl (const_gid t i0) = ret gvb ->
+  const2GV TD Mem0 gl
+         (const_gep false (const_gid t i0)
+            (Cons_list_const (const_int Size.ThirtyTwo 1) Nil_list_const)) =
+       ret gve ->
+  wf_data TD Mem0 gvb gve.
+Proof.
+  intros TD Mem0 gl t i0 gvb gve H2 H3.
+  unfold const2GV in H3.
+  remember (_const2GV TD Mem0 gl
+           (const_gep false (const_gid t i0)
+              (Cons_list_const (const_int Size.ThirtyTwo 1) Nil_list_const))) 
+    as R0.
+  destruct R0; try solve [inversion H3].
+  destruct p. inv H3.
+  unfold const2GV in H2.
+  remember (_const2GV TD Mem0 gl (const_gid t i0)) as R1.
+  destruct R1; try solve [inversion H2].
+  destruct p. inv H2.
+  unfold _const2GV in *.
+  remember (Constant.getTyp (const_gid t i0)) as R.
+  destruct R; try solve [inversion HeqR0].
+  destruct t2; try solve [inversion HeqR0].
+  remember (lookupAL GenericValue gl i0) as R'.
+  destruct R'; try solve [inversion HeqR0].
+  inv HeqR1.
+  remember (Constant.getTyp
+    (const_gep false (const_gid t i0)
+      (Cons_list_const (const_int Size.ThirtyTwo 1) Nil_list_const))) as R1.
+  destruct R1; try solve [inversion HeqR0].
+  remember (GV2ptr TD (getPointerSize TD) g) as R2.
+  destruct R2; try solve [inversion HeqR0].
+  remember (intConsts2Nats TD
+    (Cons_list_const (const_int Size.ThirtyTwo 1) Nil_list_const)) as R3.
+  destruct R3; try solve [inversion HeqR0].
+  remember (mgep TD t2 v l0) as R4.
+  destruct R4; inv HeqR0.
+  simpl in *.
+  inv HeqR3. inv HeqR. inv HeqR1.
+  admit.
+Qed.
+
+Lemma wf_rmetadata__get_const_metadata : forall TD gl Mem0 rm c gvb gve c0 c1,
+  wf_rmetadata TD Mem0 rm ->
+  get_const_metadata c = Some (c0,c1) ->
+  const2GV TD Mem0 gl c0 = Some gvb ->
+  const2GV TD Mem0 gl c1 = Some gve ->
+  wf_data TD Mem0 gvb gve.
+Proof.
+  induction c; intros gvb gve cc0 cc1 Hwfr H1 H2 H3; try solve [inversion H1].
+  destruct t; inv H1; 
+    try solve [ eauto using wf_rmetadata__get_const_metadata_aux ].
+
+    unfold const2GV in H2, H3.
+    remember (_const2GV TD Mem0 gl (const_gid (typ_function t l0) i0)) as R.
+    destruct R; try solve [inversion H2 | inversion H3].
+    destruct p. inv H2. inv H3.
+    admit. (* fptr, we should change opsem of call to check *)
+
+    simpl in H1; eauto.
+Qed.
+
+Lemma null_is_wf_data : forall TD Mem,
+  wf_data TD Mem null null.
+Proof.
+  intros TD Mem.
+  unfold wf_data.
+Admitted.
+
 Lemma wf_rmetadata__get_reg_metadata : forall TD Mem0 rm gl vp gvb gve,
   wf_rmetadata TD Mem0 rm ->
-  get_reg_metadata TD Mem0 gl rm vp = Some (mkMD gvb gve) ->
+  get_reg_metadata TD Mem0 gl rm vp = mkMD gvb gve ->
   wf_data TD Mem0 gvb gve.
 Proof.
   intros TD Mem0 rm gl vp gvb gve Hwfr J.
   unfold get_reg_metadata in J.
   destruct vp.
-    apply Hwfr in J; auto.
+    remember (lookupAL metadata rm i0) as R.
+    destruct R; inversion J; subst; auto using null_is_wf_data.
+      symmetry in HeqR.
+      apply Hwfr in HeqR; auto.
 
     remember (get_const_metadata c) as R.
-    destruct R; try solve [inversion J].
+    destruct R; try solve [inversion J; subst; auto using null_is_wf_data].
     destruct p.
     remember (const2GV TD Mem0 gl c0) as R0.
     remember (const2GV TD Mem0 gl c1) as R1.
-    destruct R0; try solve [inversion J]. simpl in J.
-    destruct R1; try solve [inversion J]. simpl in J.
+    destruct R0; try solve [inversion J; subst; auto using null_is_wf_data]. 
+    simpl in J.
+    destruct R1; try solve [inversion J; subst; auto using null_is_wf_data]. 
+    simpl in J.
     inv J.
-    unfold wf_data.
-Admitted.
+    eapply wf_rmetadata__get_const_metadata; eauto.
+Qed.
+
+Lemma wf_mmetadata__get_mem_metadata : forall TD Mem0 MM gvp gvb gve,
+  wf_mmetadata TD Mem0 MM ->
+  get_mem_metadata TD MM gvp = mkMD gvb gve ->
+  wf_data TD Mem0 gvb gve.
+Proof.
+  intros TD Mem0 MM gvp gvb gve Hwfm H4.
+  unfold get_mem_metadata in H4.
+  remember (GV2ptr TD (getPointerSize TD) gvp) as R.
+  destruct R; try solve [inversion H4; subst; auto using null_is_wf_data].
+  destruct v; try solve [inversion H4; subst; auto using null_is_wf_data].
+  remember (MM b i0) as R'.
+  destruct R'; inv H4; auto using null_is_wf_data.
+  symmetry in HeqR'.     
+  apply Hwfm in HeqR'; auto.
+Qed.
 
 Lemma dbCmd_preservation : forall TD lc rm als gl Mem MM c lc' rm' als' Mem' MM' 
     tr r, 
@@ -165,11 +257,11 @@ Case "dbMalloc".
         unfold Mem.range_perm in J2.
         apply Mem.perm_implies with (p1:=Freeable); auto with mem.
         apply J2.
-        simpl. unfold bytesize_chunk. admit.
+        simpl. unfold bytesize_chunk. admit. (*zarith*)
 
-        admit. 
-        simpl. unfold bytesize_chunk. admit.
-        simpl. unfold bytesize_chunk. admit.
+        admit. (*zarith*)
+        simpl. unfold bytesize_chunk. admit. (*zarith*)
+        simpl. unfold bytesize_chunk. admit. (*zarith*)
       
 
        rewrite <- lookupAL_updateAddAL_neq in J; auto.
@@ -191,7 +283,7 @@ Case "dbMalloc".
     destruct (zeq b0 b1); eauto using range_perm_alloc_other.
 
 Case "dbFree".
-  admit.
+  admit. (* goal is false*)
 
 Case "dbAlloca".
   invert_prop_reg_metadata. clear H3.
@@ -220,11 +312,11 @@ Case "dbAlloca".
         unfold Mem.range_perm in J2.
         apply Mem.perm_implies with (p1:=Freeable); auto with mem.
         apply J2.
-        simpl. unfold bytesize_chunk. admit.
+        simpl. unfold bytesize_chunk. admit. (*zarith*)
 
-        admit. 
-        simpl. unfold bytesize_chunk. admit.
-        simpl. unfold bytesize_chunk. admit.
+        admit.  (*zarith*)
+        simpl. unfold bytesize_chunk. admit. (*zarith*)
+        simpl. unfold bytesize_chunk. admit. (*zarith*)
       
 
        rewrite <- lookupAL_updateAddAL_neq in J; auto.
@@ -254,11 +346,7 @@ Case "dbLoad_ptr".
       clear Hwfr.
       rewrite lookupAL_updateAddAL_eq in J.
       inversion J; subst. clear J.
-      unfold get_mem_metadata in H4.
-      remember (GV2ptr TD (getPointerSize TD) gvp) as R.
-      destruct R; try solve [inversion H4].
-      destruct v; try solve [inversion H4].
-      apply Hwfm in H4; auto.
+      eapply wf_mmetadata__get_mem_metadata in H4; eauto.
 
       clear Hwfm.
       rewrite <- lookupAL_updateAddAL_neq in J; auto.
@@ -395,8 +483,425 @@ Case "dbSelect_ptr".
         rewrite <- lookupAL_updateAddAL_neq in J; auto.
         apply Hwfr in J; auto.
 
-Case "dbLib". admit.
-Case "dbLib_error". admit.
+Case "dbLib". admit. (* goal is false *)
+Case "dbLib_error". admit. (* goal is false *)
+Qed.
+
+Lemma dbCmds_preservation : forall TD lc rm als gl Mem MM cs lc' rm' als' Mem' 
+    MM' tr r,
+  SoftBound.dbCmds TD gl lc rm als Mem MM cs lc' rm' als' Mem' MM' tr r ->
+  wf_metadata TD Mem rm MM ->
+  wf_metadata TD Mem' rm' MM'.
+Proof.
+  intros TD lc rm als gl Mem MM cs lc' rm' als' Mem' MM' tr r H.
+  (sb_dbCmds_cases (induction H) Case); intros J; subst;
+    try solve [invert_result | eauto using dbCmd_preservation].
+Qed.
+
+Lemma initRmetadata_aux__wf_metadata : forall TD Mem0 gl la lp rm accum rm0 MM,
+  initRmetadata_aux TD Mem0 gl la lp rm accum = ret rm0 ->
+  wf_metadata TD Mem0 rm MM ->
+  wf_metadata TD Mem0 accum MM ->
+  wf_metadata TD Mem0 rm0 MM.
+Proof.
+  induction la; intros lp rm accum rm0 MM H Hwf; simpl in H.
+    destruct lp; inv H; auto.
+
+    destruct a.
+    destruct lp; inv H; auto.
+    destruct p.
+    destruct (isPointerTypB t); eauto.
+    remember (get_reg_metadata TD Mem0 gl rm v) as R.
+    destruct R; try solve [inv H1].
+      intro Hwf'.
+      apply IHla with (MM:=MM) in H1; auto.
+      destruct Hwf' as [Hwfr' Hwfm'].
+      destruct Hwf as [Hwfr Hwfm].
+      split; auto.
+        intros i gvb gve J.
+        destruct (@id_dec i0 i); subst.
+          rewrite lookupAL_updateAddAL_eq in J.
+          inversion J; subst. clear J.
+          symmetry in HeqR.
+          eapply wf_rmetadata__get_reg_metadata in HeqR; eauto. 
+
+          rewrite <- lookupAL_updateAddAL_neq in J; auto.
+          apply Hwfr' in J; auto.
+Qed.
+
+Lemma initRmetadata__wf_metadata : forall TD Mem0 gl la lp rm rm0 MM,
+  initRmetadata TD Mem0 gl la lp rm = ret rm0 ->
+  wf_metadata TD Mem0 rm MM ->
+  wf_metadata TD Mem0 rm0 MM.
+Proof.
+  intros TD Mem0 gl la lp rm rm0 MM H Hwf.
+  unfold initRmetadata in H.
+  eapply initRmetadata_aux__wf_metadata in H; eauto.
+  destruct Hwf as [Hwfr Hwfm].
+  split; auto.
+    intros i gvb gve J.
+    inversion J.
+Qed.
+
+Definition dbCall_preservation_prop S TD Ps fs gl lc rm Mem0 MM0 call0 lc' rm' 
+  Mem' MM' tr r 
+(db:SoftBound.dbCall S TD Ps fs gl lc rm Mem0 MM0 call0 lc' rm' Mem' MM' tr r) :=
+  wf_metadata TD Mem0 rm MM0 ->
+  wf_metadata TD Mem' rm' MM'.
+
+Definition dbSubblock_preservation_prop S TD Ps fs gl lc rm als Mem MM cs lc' rm'
+  als' Mem' MM' tr r
+(db:SoftBound.dbSubblock S TD Ps fs gl lc rm als Mem MM cs lc' rm' als' Mem' MM' 
+    tr r) :=
+  wf_metadata TD Mem rm MM ->
+  wf_metadata TD Mem' rm' MM'.
+
+Definition dbSubblocks_preservation_prop S TD Ps fs gl lc rm als Mem MM cs lc' 
+  rm' als' Mem' MM' tr r 
+(db:SoftBound.dbSubblocks S TD Ps fs gl lc rm als Mem MM cs lc' rm' als' Mem' MM'
+  tr r) :=
+  wf_metadata TD Mem rm MM ->
+  wf_metadata TD Mem' rm' MM'.
+
+Definition dbBlock_preservation_prop S TD Ps fs gl F state state' tr r
+  (db:SoftBound.dbBlock S TD Ps fs gl F state state' tr r) :=
+  forall l ps cs tmn lc rm als Mem MM l' ps' cs' tmn' lc' rm' als' Mem' MM',
+  state = SoftBound.mkState (SoftBound.mkEC (block_intro l ps cs tmn) lc rm als)
+    Mem MM ->
+  state' = SoftBound.mkState (SoftBound.mkEC (block_intro l' ps' cs' tmn') lc' 
+    rm' als') Mem' MM' ->
+  wf_metadata TD Mem rm MM ->
+  wf_metadata TD Mem' rm' MM'.
+
+Definition dbBlocks_preservation_prop S TD Ps fs gl F state state' tr r
+  (db:SoftBound.dbBlocks S TD Ps fs gl F state state' tr r) :=
+  forall l ps cs tmn lc rm als Mem MM l' ps' cs' tmn' lc' rm' als' Mem' MM',
+  state = SoftBound.mkState (SoftBound.mkEC (block_intro l ps cs tmn) lc rm als)
+    Mem MM ->
+  state' = SoftBound.mkState (SoftBound.mkEC (block_intro l' ps' cs' tmn') lc' 
+    rm' als') Mem' MM' ->
+  wf_metadata TD Mem rm MM ->
+  wf_metadata TD Mem' rm' MM'.
+
+Definition dbFdef_preservation_prop fid rt lp S TD Ps lc rm gl fs Mem MM lc'
+  rm' als' Mem' MM' B' Rid oResult tr r
+  (db:SoftBound.dbFdef fid rt lp S TD Ps lc rm gl fs Mem MM lc' rm' als' Mem' MM'
+    B' Rid oResult tr r) :=
+  wf_metadata TD Mem rm MM ->
+  wf_metadata TD Mem' rm' MM'.
+
+Lemma sbop_preservation :
+  (forall S TD Ps fs gl lc rm Mem0 MM0 call0 lc' rm' Mem' MM' tr r db, 
+     dbCall_preservation_prop S TD Ps fs gl lc rm Mem0 MM0 call0 lc' rm' 
+       Mem' MM' tr r db) 
+    /\
+  (forall S TD Ps fs gl lc rm als Mem MM sb lc' rm' als' Mem' MM' tr r db,
+     dbSubblock_preservation_prop S TD Ps fs gl lc rm als Mem MM sb lc' 
+       rm' als' Mem' MM' tr r db) /\
+  (forall S TD Ps fs gl lc rm als Mem MM sbs lc' rm' als' Mem' MM' tr r db,
+     dbSubblocks_preservation_prop S TD Ps fs gl lc rm als Mem MM sbs 
+       lc' rm' als' Mem' MM' tr r db) /\
+  (forall S TD Ps fs gl F state1 state2 tr r db,
+     dbBlock_preservation_prop S TD Ps fs gl F state1 state2 tr r db) /\
+  (forall S TD Ps fs gl F state1 state2 tr r db,
+     dbBlocks_preservation_prop S TD Ps fs gl F state1 state2 tr r db) /\
+  (forall fid rt lp S1 TD Ps1 lc rm gl fs Mem MM lc' rm' als' Mem' MM' B' Rid 
+       oResult tr r db,
+     dbFdef_preservation_prop fid rt lp S1 TD Ps1 lc rm gl fs Mem MM lc' rm'
+       als' Mem' MM' B' Rid oResult tr r db).
+Proof.
+(sb_db_mutind_cases
+  apply SoftBound.sb_db_mutind with
+    (P  := dbCall_preservation_prop)
+    (P0 := dbSubblock_preservation_prop)
+    (P1 := dbSubblocks_preservation_prop)
+    (P2 := dbBlock_preservation_prop)
+    (P3 := dbBlocks_preservation_prop)
+    (P4 := dbFdef_preservation_prop) Case);
+  unfold dbCall_preservation_prop, 
+         dbFdef_preservation_prop, dbSubblock_preservation_prop,
+         dbSubblocks_preservation_prop, 
+         dbBlock_preservation_prop,
+         dbBlocks_preservation_prop; intros; subst; 
+    try solve [ eauto using dbCmds_preservation ].
+Case "dbCall_internal". admit. (* goal is false *)
+Case "dbCall_external". admit. (* goal is false *)
+Case "dbCall_internal_error1". admit. (* goal is false *)
+Case "dbCall_external_error1". admit. (* goal is false *)
+
+Case "dbBlock_ok".
+  inv H1. inv H0.
+  apply dbCmds_preservation in d0; eauto.
+
+Case "dbBlock_error1".
+  inv H1. inv H0. eauto.
+  apply dbCmds_preservation in d0; eauto.
+
+Case "dbBlock_error2".
+  inv H1. inv H0. eauto.
+
+Case "dbBlocks_nil".
+  inv H0. auto.
+
+Case "dbBlocks_cons".
+  inversion d; subst; try solve [ invert_result ].
+  destruct B'. eauto.
+
+Case "dbBlocks_cons_error".
+  inv H1. eauto.
+  destruct B2. eauto.
+
+Case "dbFdef_func".
+  apply dbCmds_preservation in d1; eauto.
+  apply H0; auto.
+  eapply H; eauto.
+  eapply initRmetadata__wf_metadata in e1; eauto.
+
+Case "dbFdef_func_error1".
+  apply H0; auto.
+  eapply H; eauto.
+  eapply initRmetadata__wf_metadata in e1; eauto.
+
+Case "dbFdef_func_error2".
+  eapply H; eauto.
+  eapply initRmetadata__wf_metadata in e1; eauto.
+
+Case "dbFdef_proc".
+  apply dbCmds_preservation in d1; eauto.
+  apply H0; auto.
+  eapply H; eauto.
+  eapply initRmetadata__wf_metadata in e1; eauto.
+
+Case "dbFdef_proc_error1".
+  apply H0; auto.
+  eapply H; eauto.
+  eapply initRmetadata__wf_metadata in e1; eauto.
+
+Case "dbFdef_proc_error2".
+  eapply H; eauto.
+  eapply initRmetadata__wf_metadata in e1; eauto.
+Qed.
+
+Require Import Znumtheory.
+
+Lemma assert_mptr_dec : forall TD t ptr md,
+  assert_mptr TD t ptr md \/ ~ assert_mptr TD t ptr md.
+Admitted.
+
+Lemma assert_mptr__valid_access : forall md TD Mem gl rm v MM t g b ofs c,
+  wf_metadata TD Mem rm MM ->
+  md = get_reg_metadata TD Mem gl rm v ->
+  assert_mptr TD t g md ->
+  GV2ptr TD (getPointerSize TD) g = ret Values.Vptr b ofs ->
+  typ2memory_chunk t = ret c ->
+  (align_chunk c | Int.unsigned 31 ofs) ->
+  Mem.valid_access Mem c b (Int.unsigned 31 ofs) Writable.
+Proof.
+  intros md TD Mem gl rm v MM t g b ofs c Hwf Heqmd J R3 R4 R5.
+      unfold Mem.valid_access.
+      split; auto.
+        unfold assert_mptr in J.
+        rewrite R3 in J.
+        symmetry in Heqmd.  
+        destruct md.
+        destruct Hwf as [Hwfr Hwfm].
+        apply wf_rmetadata__get_reg_metadata in Heqmd; auto.
+        unfold wf_data in Heqmd.
+        destruct (GV2ptr TD (getPointerSize TD) md_base0); 
+          try solve [inversion Heqmd].
+        destruct v0; try solve [inversion Heqmd].
+        destruct (GV2ptr TD (getPointerSize TD) md_bound0); 
+          try solve [inversion Heqmd].
+        destruct v0; try solve [inversion Heqmd].
+        destruct (zeq b0 b1); subst; try solve [inversion Heqmd].
+        remember (getTypeAllocSize TD t) as R6.
+        destruct R6; try solve [inversion J].
+        simpl in J.
+        intros z Jz.
+        destruct J as [J1 [_ [J2 J3]]].
+        destruct (zeq b b1); subst; try solve [inversion J1].
+        apply Heqmd.
+        clear - J2 J3 Jz HeqR6 R4.
+        admit.        
+Qed.
+
+Lemma dbCmd_progress : forall TD lc rm als gl Mem MM c, 
+  wf_metadata TD Mem rm MM ->
+  SimpleSE.isCall c = false ->
+  exists lc', exists rm', exists als', exists Mem', exists MM', exists tr, 
+  exists r, 
+    dbCmd TD gl lc rm als Mem MM c lc' rm' als' Mem' MM' tr r.
+Proof.
+  intros TD lc rm als gl Mem MM c Hwf Hiscall.
+  cmd_cases (destruct c) Case.
+
+Case "insn_bop".
+  remember (BOP TD Mem lc gl b s v v0) as R.
+  destruct R.
+    exists (updateAddAL _ lc i0 g). exists rm. exists als. exists Mem.
+    exists MM. exists trace_nil. exists rok.
+    apply dbBop; auto.
+
+    exists lc. exists rm. exists als. exists Mem. exists MM. exists trace_nil. 
+    exists rerror.
+    apply dbBop_error; auto.
+
+admit. admit. admit.
+admit. admit. admit.
+
+Case "insn_load".
+
+  assert (exists g, getOperandValue TD Mem v lc gl = Some g) as R2.
+    admit. (* wont be stuck for well-formed SSA. *)
+  destruct R2 as [g R2].
+  remember (isPointerTypB t) as R1.
+  remember (get_reg_metadata TD Mem gl rm v) as md.
+  destruct (assert_mptr_dec TD t g md) as [J | J].
+  SCase "assert ok".
+    assert (exists b, exists ofs, 
+      GV2ptr TD (getPointerSize TD) g = Some (Values.Vptr b ofs)) as R3. 
+      admit. (* from wf *)
+    assert (exists c, typ2memory_chunk t = Some c) as R4. 
+      admit. (* from wf *)
+    destruct R3 as [b [ofs R3]].
+    destruct R4 as [c R4].
+    destruct (Zdivide_dec (align_chunk c) (Int.unsigned 31 ofs)) as [R5 | R5].
+    SSCase "align ok".
+      assert (exists gv, mload TD Mem g t a = Some gv) as R6.
+        unfold mload.
+        rewrite R3. rewrite R4.
+        assert (Mem.valid_access Mem c b (Int.unsigned 31 ofs) Readable) as J'.
+          apply Mem.valid_access_implies with (p1:=Writable); auto with mem.
+          eapply assert_mptr__valid_access; eauto.
+        apply Mem.valid_access_load in J'.
+        destruct J' as [v0 J'].
+        rewrite J'.
+        exists (val2GV TD v0 c). auto.
+      destruct R6 as [gv R6].
+      destruct R1.
+      SSSCase "t is ptr".
+        remember (prop_reg_metadata lc rm i0 gv (get_mem_metadata TD MM g)) 
+          as R7.
+        destruct R7 as (lc', rm'). 
+        subst.
+        exists lc'. exists rm'. exists als. exists Mem. exists MM. 
+        exists trace_nil. exists rok. eapply dbLoad_ptr; eauto.
+        unfold isPointerTyp. auto.
+      SSSCase "t isnt ptr".
+        subst.
+        exists (updateAddAL _ lc i0 gv). exists rm. exists als. exists Mem. 
+        exists MM. exists trace_nil. exists rok. eapply dbLoad_nptr; eauto.
+        unfold isPointerTyp. rewrite <- HeqR1. intro JJ. inversion JJ.
+    SSCase "align fails".
+      subst.
+      exists lc. exists rm. exists als. exists Mem. exists MM. exists trace_nil.
+      exists rerror. eapply dbLoad_error3; eauto.
+  SCase "assert fails".
+    subst.
+    exists lc. exists rm. exists als. exists Mem. exists MM. exists trace_nil.
+     exists rabort. eapply dbLoad_abort; eauto.
+
+Case "insn_store".
+
+  assert (exists gv, getOperandValue TD Mem v lc gl = Some gv) as R21.
+    admit. (* wont be stuck for well-formed SSA. *)
+  assert (exists gvp, getOperandValue TD Mem v0 lc gl = Some gvp) as R22.
+    admit. (* wont be stuck for well-formed SSA. *)
+  destruct R21 as [gv R21].
+  destruct R22 as [gvp R22].
+  remember (isPointerTypB t) as R1.
+  remember (get_reg_metadata TD Mem gl rm v0) as md.
+  destruct (assert_mptr_dec TD t gvp md) as [J | J].
+  SCase "assert ok".
+    assert (exists b, exists ofs, 
+      GV2ptr TD (getPointerSize TD) gvp = Some (Values.Vptr b ofs)) as R3. 
+      admit. (* from wf *)
+    assert (exists c, typ2memory_chunk t = Some c) as R4. 
+      admit. (* from wf *)
+    destruct R3 as [b [ofs R3]].
+    destruct R4 as [c R4].
+    assert (exists v1, GV2val TD gv = Some v1) as R8.
+      admit. (* ?!? *)
+    assert (exists v2, GV2val TD gvp = Some v2) as R9.
+      admit. (* ?!? *)
+    destruct R8 as [v1 R8].
+    destruct R9 as [v2 R9].
+    destruct (Zdivide_dec (align_chunk c) (Int.unsigned 31 ofs)) as [R5 | R5].
+    SSCase "align ok".
+      assert (exists Mem', mstore TD Mem gvp t gv a = Some Mem') as R6.
+        unfold mstore.
+        rewrite R3. rewrite R4.
+        assert (Mem.valid_access Mem c b (Int.unsigned 31 ofs) Writable) as J'.
+          eapply assert_mptr__valid_access; eauto.
+        assert (J2:=@Mem.valid_access_store Mem c b (Int.unsigned 31 ofs) v1 J').
+        destruct J2 as [Mem' J2].
+        rewrite R8.
+        exists Mem'. auto.
+      destruct R6 as [Mem' R6].
+      destruct R1.
+      SSSCase "t is ptr".
+        subst.
+        exists lc. exists rm. exists als. exists Mem'. 
+        exists (set_mem_metadata TD MM gvp (get_reg_metadata TD Mem gl rm v)). 
+        exists trace_nil. exists rok. 
+        eapply dbStore_ptr; eauto.
+          unfold isPointerTyp. auto.
+      SSSCase "t isnt ptr".
+        subst.
+        exists lc. exists rm. exists als. exists Mem'. exists MM. 
+        exists trace_nil. exists rok. 
+        eapply dbStore_nptr; eauto.
+          unfold isPointerTyp. rewrite <- HeqR1. intro JJ. inversion JJ.
+    SSCase "align fails".
+      subst.
+      exists lc. exists rm. exists als. exists Mem. exists MM. exists trace_nil.
+      exists rerror. eapply dbStore_error3; eauto.
+  SCase "assert fails".
+    subst.
+    exists lc. exists rm. exists als. exists Mem. exists MM. exists trace_nil.
+     exists rabort. eapply dbStore_abort; eauto.
+
+Case "insn_gep".
+
+Admitted.
+
+Fixpoint NonCallCmds (cs:cmds) : Prop :=
+match cs with
+| nil => True
+| c::cs' => SimpleSE.isCall c = false /\ NonCallCmds cs'
+end.
+
+Lemma dbCmds_progress : forall cs TD lc rm als gl Mem MM, 
+  wf_metadata TD Mem rm MM ->
+  NonCallCmds cs ->
+  exists lc', exists rm', exists als', exists Mem', exists MM', exists tr, 
+  exists r, 
+    dbCmds TD gl lc rm als Mem MM cs lc' rm' als' Mem' MM' tr r.
+Proof.
+  induction cs; intros.
+    exists lc. exists rm. exists als. exists Mem0. exists MM. exists trace_nil.
+    exists rok.
+    apply dbCmds_nil.
+
+    simpl in H0.
+    destruct H0 as [J1 J2].
+    assert (Hwfm:=H).
+    apply dbCmd_progress with (lc:=lc)(gl:=gl)(c:=a)(als:=als) in H; auto.
+    destruct H as [lc' [rm' [als' [Mem' [MM' [tr [r H]]]]]]].
+    destruct r.
+      assert (J3:=H).
+      apply dbCmd_preservation in J3; auto.
+      assert (J:=@IHcs TD lc' rm' als' gl Mem' MM' J3 J2).
+      destruct J as [lc'' [rm'' [als'' [Mem'' [MM'' [tr' [r' J]]]]]]].
+      exists lc''. exists rm''. exists als''. exists Mem''. exists MM''. 
+      exists (trace_app tr tr'). exists r'. 
+      eapply dbCmds_cons; simpl; eauto.
+
+      exists lc'. exists rm'. exists als'. exists Mem'. exists MM'. exists tr. 
+      exists rabort. apply dbCmds_cons_error; simpl; auto.
+
+      exists lc'. exists rm'. exists als'. exists Mem'. exists MM'. exists tr. 
+      exists rerror. apply dbCmds_cons_error; simpl; auto.
 Qed.
 
 (*****************************)
